fix intervals during insertion

src/Insert.v
@@ -18,6 +18,86 @@ Section nary_tree.
                     else target :: x :: xs
     end.
 
+    Fixpoint insert_nary_tree_spec (target : Z) (t : nary_tree) : nary_tree * option nary_tree :=
+      match t with
+      | leaf (low, high) vals =>
+          let new_vals := insert_list_spec target vals in
+          if Z.ltb b (length new_vals)
+          then
+            let left_vals := firstn (b/2) new_vals in
+            let right_vals := skipn (b/2) new_vals in
+            let left_interval := (hd low left_vals, List.last left_vals high) in
+            let right_interval := (hd low right_vals, List.last right_vals high) in
+            (leaf left_interval left_vals, Some (leaf right_interval right_vals))
+          else
+            (leaf (hd low new_vals, List.last new_vals high) new_vals, None)
+      | node (low, high) branches =>
+          let new_branches :=
+            ((fix insert_aux (l : list nary_tree) :=
+                match l with
+                | [] => []
+                | t :: [] =>
+                    let (new_t1, new_t2) := insert_nary_tree_spec target t in
+                    match new_t2 with
+                    | None => [new_t1]
+                    | Some new_t2' => new_t1 :: [new_t2']
+                    end
+                | t :: ts =>
+                    let (low, high) := nary_tree_interval t in
+                    if andb (Z.leb low target) (Z.leb target high)
+                    then let (new_t1, new_t2) := insert_nary_tree_spec target t in
+                         match new_t2 with
+                         | None => new_t1 :: ts
+                         | Some new_t2' => new_t1 :: new_t2' :: ts
+                         end
+                    else t :: insert_aux ts
+                end) branches) in
+          if Z.ltb b (length new_branches)
+          then
+            let left_branches := firstn (b/2) new_branches in
+            let right_branches := skipn (b/2) new_branches in
+            let left_interval_low :=
+              match head (map fst (map nary_tree_interval left_branches)) with
+              | None => low
+              | Some x => x
+              end
+            in
+            let left_interval_high :=
+              match last (map snd (map nary_tree_interval left_branches)) with
+              | None => high
+              | Some x => x
+              end
+            in
+            let right_interval_low :=
+              match head (map fst (map nary_tree_interval right_branches)) with
+              | None => low
+              | Some x => x
+              end
+            in
+            let right_interval_high :=
+              match last (map snd (map nary_tree_interval right_branches)) with
+              | None => high
+              | Some x => x
+              end
+            in
+            (node (left_interval_low, left_interval_high) left_branches,
+              Some (node (right_interval_low, right_interval_high) right_branches))
+          else
+            let new_low :=
+              match head (map fst (map nary_tree_interval new_branches)) with
+              | None => low
+              | Some x => x
+              end
+            in
+            let new_high :=
+              match last (map snd (map nary_tree_interval new_branches)) with
+              | None => high
+              | Some x => x
+              end
+            in
+            (node (new_low, new_high) new_branches, None)
+      end.
+
   (* Definition insert_bplus_tree_spec (target : Z) (t : bplus_tree) := *)
   (*   match t with *)
   (*   | root_leaf (low, high) vals => *)
@@ -105,6 +185,151 @@ Section bplus_tree.
               "l" <- ("x", Fst "rec") ;;
               (SOME "l", Snd "rec")
           end.
+
+    Definition head_list : val :=
+      rec: "head_list" "arg" :=
+        match: Fst "arg" with
+          NONE => Snd "arg"
+        | SOME "l" => Fst !"l"
+        end.
+
+    Definition last_list : val :=
+      rec: "last_list" "arg" :=
+        match: Fst "arg" with
+          NONE => Snd "arg"
+        | SOME "l" =>
+            match: Snd !"l" with
+              NONE => Fst !"l"
+            | SOME "l'" => "last_list" (SOME "l'", Snd "arg")
+            end
+        end.
+
+    Definition headopt_list : val :=
+      rec: "headopt_list" "l" :=
+        match: "l" with
+          NONE => NONE
+        | SOME "l" => SOME (Fst !"l")
+        end.
+
+    Definition lastopt_list : val :=
+      rec: "lastopt_list" "l" :=
+        match: "l" with
+          NONE => NONE
+        | SOME "l" =>
+            match: Snd !"l" with
+              NONE => SOME (Fst !"l")
+            | SOME "l'" => "lastopt_list" (SOME "l'")
+            end
+        end.
+
+    Definition interval_nary_tree : val :=
+      rec: "interval_nary_tree" "t" :=
+        match: "t" with
+          InjL "ptr" => Fst !"ptr"
+        | InjR "ptr" => Fst !"ptr"
+        end.
+
+    Definition insert_nary_tree : val :=
+      rec: "insert_nary_tree" "arg" :=
+        let: "t" := Fst "arg" in
+        let: "target" := Snd "arg" in
+        match: "t" with
+          InjL "ptr" =>
+            let: "lhd" := Snd !"ptr" in
+            let: "interval" := Fst !"ptr" in
+            let: "new" := insert_list ("lhd", "target") in
+            if: #b < length_list "new"
+            then
+              let: "newlpair" := split_list ("new", #(b/2)) in
+              let: "newhead1" := head_list (Fst "newlpair", Fst "interval") in
+              let: "newlast1" := last_list (Fst "newlpair", Snd "interval") in
+              let: "newhead2" := head_list (Snd "newlpair", Fst "interval") in
+              let: "newlast2" := last_list (Snd "newlpair", Snd "interval") in
+              let: "newleaf" := ref (("newhead2", "newlast2"), Snd "newlpair") in
+              "ptr" <- (("newhead1", "newlast1"), Fst "newlpair") ;;
+              (token_leaf_e "ptr", SOME (token_leaf_e "newleaf"))
+            else
+              let: "head" := head_list ("new", Fst "interval") in
+              let: "last" := last_list ("new", Snd "interval") in
+              "ptr" <- (("head", "last"), "new") ;;
+              (token_leaf_e "ptr", NONEV)
+        | InjR "ptr" =>
+            let: "lhd" := Snd !"ptr" in
+            let: "new" :=
+              (rec: "insert_node_list" "arg" :=
+                 let: "p" := Fst "arg" in
+                 let: "target" := Snd "arg" in
+                 match: "p" with
+                   NONE =>
+                     NONE
+                 | SOME "l" =>
+                     match: Snd !"l" with
+                       NONE =>
+                         let: "newt" := "insert_nary_tree" (Fst !"l", "target") in
+                         match: Snd "newt" with
+                           NONE => "l" <- (Fst "newt", NONE)
+                         | SOME "newt2" =>
+                             let: "l'" := ref ("newt2", NONE) in
+                             "l" <- (Fst "newt", SOME "l'")
+                         end
+                     | SOME "_" =>
+                         let: "thd" := Fst !"l" in
+                         let: "interval" := interval_nary_tree "thd" in
+                         let: "low" := Fst "interval" in
+                         let: "high" := Snd "interval" in
+                         (if: (BinOp LeOp "low" "target") && (BinOp LeOp "target" "high")
+                          then let: "newt" := "insert_nary_tree" ("thd", "target") in
+                               match: Snd "newt" with
+                                 NONE => "l" <- (Fst "newt", Snd !"l")
+                               | SOME "newt2" =>
+                                   let: "l'" := ref ("newt2", Snd !"l") in
+                                   "l" <- (Fst "newt", SOME "l'")
+                               end
+                          else let: "newl" := "insert_node_list" (Snd !"l", "target") in
+                               "l" <- ("thd", "newl"))
+                     end ;; SOME "l"
+                 end) ("lhd", "target") in
+            let: "interval" := Fst !"ptr" in
+            if: #b < length_list "new"
+            then
+              let: "newlpair" := split_list ("new", #(b/2)) in
+              let: "newheadleft" :=
+                match: headopt_list (Fst "newlpair") with
+                  NONE => Fst "interval"
+                | SOME "t" => Fst (interval_nary_tree "t")
+                end in
+              let: "newlastleft" :=
+                match: lastopt_list (Fst "newlpair") with
+                  NONE => Snd "interval"
+                | SOME "t" => Snd (interval_nary_tree "t")
+                end in
+              let: "newheadright" :=
+                match: headopt_list (Snd "newlpair") with
+                  NONE => Fst "interval"
+                | SOME "t" => Fst (interval_nary_tree "t")
+                end in
+              let: "newlastright" :=
+                match: lastopt_list (Snd "newlpair") with
+                  NONE => Snd "interval"
+                | SOME "t" => Snd (interval_nary_tree "t")
+                end in
+              let: "newbranch" := ref (("newheadright", "newlastright"), Snd "newlpair") in
+              "ptr" <- (("newheadleft", "newlastleft"), Fst "newlpair") ;;
+              (token_branch_e "ptr", SOME (token_branch_e "newbranch"))
+            else
+              let: "newhead" :=
+                match: headopt_list "new" with
+                  NONE => Fst "interval"
+                | SOME "t" => Fst (interval_nary_tree "t")
+                end in
+              let: "newlast" :=
+                match: lastopt_list "new" with
+                  NONE => Snd "interval"
+                | SOME "t" => Snd (interval_nary_tree "t")
+                end in
+              "ptr" <- (("newhead", "newlast"), "new") ;;
+              (token_branch_e "ptr", NONEV)
+        end%E.
 
   End bplus_tree_algos.
 
@@ -244,122 +469,113 @@ Section bplus_tree.
           done.
     Qed.
 
-  Fixpoint insert_nary_tree_spec (target : Z) (t : nary_tree) : nary_tree * option nary_tree :=
-    match t with
-    | leaf (low, high) vals =>
-        let new_vals := insert_list_spec target vals in
-        if Z.ltb b (length new_vals)
-        then
-          let left_vals := firstn (b/2) new_vals in
-          let right_vals := skipn (b/2) new_vals in
-          let left_interval := (low, List.last left_vals high) in
-          let right_interval := (hd low right_vals, high) in
-          (* TODO: fix interval *)
-          (leaf (low, high) left_vals, Some (leaf (low, high) right_vals))
-        else
-          (leaf (low, high) new_vals, None)
-    | node (low, high) branches =>
-        let new_branches :=
-          ((fix insert_aux (l : list nary_tree) :=
-              match l with
-              | [] => []
-              | t :: [] =>
-                  let (new_t1, new_t2) := insert_nary_tree_spec target t in
-                  match new_t2 with
-                  | None => [new_t1]
-                  | Some new_t2' => new_t1 :: [new_t2']
-                  end
-              | t :: ts =>
-                  let (low, high) := (match t with leaf interval _ | node interval _ => interval end) in
-                  if andb (Z.leb low target) (Z.leb target high)
-                  then let (new_t1, new_t2) := insert_nary_tree_spec target t in
-                       match new_t2 with
-                       | None => new_t1 :: ts
-                       | Some new_t2' => new_t1 :: new_t2' :: ts
-                       end
-                  else t :: insert_aux ts
-              end) branches) in
-        if Z.ltb b (length new_branches)
-        then
-          let left_branches := firstn (b/2) new_branches in
-          let right_branches := skipn (b/2) new_branches in
-          let left_interval := (low, (List.last (map snd (map nary_tree_interval left_branches)) high)) in
-          let right_interval := (hd low (map fst (map nary_tree_interval right_branches)), high) in
-          (* TODO: should change intervals *)
-          (node (low, high) left_branches, Some (node (low, high) right_branches))
-        else
-          (node (low, high) new_branches, None)
-    end.
+    Lemma head_list_spec_proof (v : val) (l : list val) (d : val):
+      {{{ is_list v l }}} head_list (v, d)%V {{{ r, RET r; ⌜r = hd d l⌝ ∗ is_list v l }}}.
+    Proof.
+      iIntros (Φ) "Hl HPost".
+      wp_lam; wp_pures.
+      destruct l as [|x l].
+      - iDestruct "Hl" as "->".
+        wp_pures.
+        iApply "HPost".
+        done.
+      - iDestruct "Hl" as (l' ?) "(-> & Hl' & Hl)".
+        wp_load; wp_pures.
+        iApply "HPost".
+        iSplitR; [done|].
+        iExists l', hd'.
+        iFrame; done.
+    Qed.
 
-    Definition insert_nary_tree : val :=
-      rec: "insert_nary_tree" "arg" :=
-        let: "t" := Fst "arg" in
-        let: "target" := Snd "arg" in
-        match: "t" with
-          InjL "ptr" =>
-            let: "lhd" := Snd !"ptr" in
-            let: "new" := insert_list ("lhd", "target") in
-            (* TODO: should change interval here *)
-            if: #b < length_list "new"
-            then
-              let: "newlpair" := split_list ("new", #(b/2)) in
-              let: "newleaf" := ref (Fst !"ptr", Snd "newlpair") in
-              "ptr" <- (Fst !"ptr", Fst "newlpair") ;;
-              (token_leaf_e "ptr", SOME (token_leaf_e "newleaf"))
-            else
-              "ptr" <- (Fst !"ptr", "new") ;;
-              (token_leaf_e "ptr", NONEV)
-        | InjR "ptr" =>
-            let: "lhd" := Snd !"ptr" in
-            let: "new" :=
-              (rec: "insert_node_list" "arg" :=
-                 let: "p" := Fst "arg" in
-                 let: "target" := Snd "arg" in
-                 match: "p" with
-                   NONE =>
-                     NONE
-                 | SOME "l" =>
-                     match: Snd !"l" with
-                       NONE =>
-                         let: "newt" := "insert_nary_tree" (Fst !"l", "target") in
-                         match: Snd "newt" with
-                           NONE => "l" <- (Fst "newt", NONE)
-                         | SOME "newt2" =>
-                             let: "l'" := ref ("newt2", NONE) in
-                             "l" <- (Fst "newt", SOME "l'")
-                         end
-                     | SOME "_" =>
-                         let: "thd" := Fst !"l" in
-                         let: "interval" :=
-                           match: "thd" with
-                             InjL "ptr" => Fst !"ptr"
-                           | InjR "ptr" => Fst !"ptr"
-                           end in
-                         let: "low" := Fst "interval" in
-                         let: "high" := Snd "interval" in
-                         (if: (BinOp LeOp "low" "target") && (BinOp LeOp "target" "high")
-                          then let: "newt" := "insert_nary_tree" ("thd", "target") in
-                               (* TODO: should change interval here *)
-                               match: Snd "newt" with
-                                 NONE => "l" <- (Fst "newt", Snd !"l")
-                               | SOME "newt2" =>
-                                   let: "l'" := ref ("newt2", Snd !"l") in
-                                   "l" <- (Fst "newt", SOME "l'")
-                               end
-                          else let: "newl" := "insert_node_list" (Snd !"l", "target") in
-                               "l" <- ("thd", "newl"))
-                     end ;; SOME "l"
-                 end) ("lhd", "target") in
-            if: #b < length_list "new"
-            then
-              let: "newlpair" := split_list ("new", #(b/2)) in
-              let: "newbranch" := ref (Fst !"ptr", Snd "newlpair") in
-              "ptr" <- (Fst !"ptr", Fst "newlpair") ;;
-              (token_branch_e "ptr", SOME (token_branch_e "newbranch"))
-            else
-              "ptr" <- (Fst !"ptr", "new") ;;
-              (token_branch_e "ptr", NONEV)
-        end%E.
+    Lemma last_list_spec_proof (v : val) (l : list val) (d : val):
+      {{{ is_list v l }}} last_list (v, d)%V {{{ r, RET r; ⌜r = List.last l d⌝ ∗ is_list v l }}}.
+    Proof.
+      iIntros (Φ) "Hl HPost".
+      iInduction l as [|x l] "IH" forall (v);
+        wp_rec; wp_pures.
+      - iDestruct "Hl" as "->".
+        wp_pures.
+        iApply "HPost".
+        iFrame; done.
+      - iDestruct "Hl" as (l' ?) "(-> & Hl' & Hl)".
+        wp_load; wp_pures.
+        destruct l as [|x' l].
+        + iDestruct "Hl" as "->".
+          wp_load; wp_pures.
+          iApply "HPost".
+          iSplitR; [done|].
+          iExists l', NONEV.
+          iFrame; done.
+        + iDestruct "Hl" as (l'' ?) "(-> & Hl'' & Hl)".
+          wp_pures.
+          iApply ("IH" with "[Hl Hl'']"); [iExists l'', hd'0; iFrame; done|].
+          iNext.
+          iIntros (?) "[-> Hl'']".
+          iApply "HPost".
+          iSplitR; [done|].
+          iExists l', (SOMEV #l'').
+          iFrame; done.
+    Qed.
+
+    Lemma headopt_list_spec_proof (v : val) (l : list val):
+      {{{ is_list v l }}} headopt_list v%V {{{ r, RET r; ⌜r = match head l with None => NONEV | Some x => SOMEV x end⌝ ∗ is_list v l }}}.
+    Proof.
+      iIntros (Φ) "Hl HPost".
+      wp_lam; wp_pures.
+      destruct l as [|x l].
+      - iDestruct "Hl" as "->".
+        wp_pures.
+        iApply "HPost".
+        done.
+      - iDestruct "Hl" as (l' ?) "(-> & Hl' & Hl)".
+        wp_load; wp_pures.
+        iApply "HPost".
+        iSplitR; [done|].
+        iExists l', hd'.
+        iFrame; done.
+    Qed.
+
+    Lemma lastopt_list_spec_proof (v : val) (l : list val):
+      {{{ is_list v l }}} lastopt_list v%V {{{ r, RET r; ⌜r = match last l with None => NONEV | Some x => SOMEV x end⌝ ∗ is_list v l }}}.
+    Proof.
+      iIntros (Φ) "Hl HPost".
+      iInduction l as [|x l] "IH" forall (v);
+        wp_lam; wp_pures.
+      - iDestruct "Hl" as "->".
+        wp_pures.
+        iApply "HPost"; done.
+      - iDestruct "Hl" as (l' ?) "(-> & Hl' & Hl)".
+        wp_load; wp_pures.
+        destruct l as [|x' l].
+        + iDestruct "Hl" as "->".
+          wp_load; wp_pures.
+          iApply "HPost".
+          iSplitR; [done|].
+          iExists l', NONEV.
+          iFrame; done.
+        + iDestruct "Hl" as (l'' ?) "(-> & Hl'' & Hl)".
+          wp_pures.
+          iApply ("IH" with "[Hl'' Hl]"); [iExists l'', hd'0; iFrame; done|].
+          iNext.
+          iIntros (?) "[% Hl'']".
+          iApply "HPost".
+          iSplitR; [done|].
+          iExists l', (SOMEV #l''); iFrame; done.
+    Qed.
+
+    Lemma interval_nary_tree_spec_proof (v : val) (t : nary_tree) :
+      {{{ is_node v t }}} interval_nary_tree v%V {{{ r, RET (#r.1, #r.2); is_node v t ∗ ⌜r = nary_tree_interval t⌝ }}}.
+      iIntros (?) "Hv HPost".
+      destruct t; destruct interval as [low high].
+      - iDestruct "Hv" as (ptr leaves) "(-> & Hptr & Hleaves)".
+        wp_rec; wp_load; wp_pures.
+        iApply ("HPost" $! (low, high)).
+        iSplitL; [iExists ptr, leaves; iFrame|]; done.
+      - iDestruct "Hv" as (ptr ns branches) "(-> & Hptr & Hns & Hbranches)".
+        wp_rec; wp_load; wp_pures.
+        iApply ("HPost" $! (low, high)).
+        iSplitL; [iExists ptr, ns, branches; iFrame|]; done.
+    Qed.
 
     Lemma branch_node_list_lengths : forall ns ts,
       (fix branch_node_list (ns0 : list val) (ts0 : list nary_tree) {struct ts0} : iProp :=
@@ -398,7 +614,7 @@ Section bplus_tree.
       done.
     Qed.
 
-    Lemma branch_node_split ns ts n :
+    Lemma branch_node_split n ns ts :
       (fix branch_node_list (ns1 : list val) (ts0 : list nary_tree) {struct ts0} : iProp :=
          match ns1 with
          | [] => match ts0 with
@@ -445,6 +661,171 @@ Section bplus_tree.
       iApply "IH"; done.
     Qed.
 
+    Lemma branch_node_snoc xs xlast ys ylast :
+      ((fix branch_node_list (ns1 : list val) (ts0 : list nary_tree) {struct ts0} :
+         iProp :=
+          match ns1 with
+          | [] => match ts0 with
+                 | [] => True%I
+                 | _ :: _ => False%I
+                 end
+          | n :: ns2 =>
+              match ts0 with
+              | [] => False%I
+              | t :: ts1 => (is_node n t ∗ branch_node_list ns2 ts1)%I
+              end
+          end) (xs ++ [xlast]) (ys ++ [ylast]) -∗
+         (fix branch_node_list (ns1 : list val) (ts0 : list nary_tree) {struct ts0} :
+           iProp :=
+            match ns1 with
+            | [] => match ts0 with
+                   | [] => True%I
+                   | _ :: _ => False%I
+                   end
+            | n :: ns2 =>
+                match ts0 with
+                | [] => False%I
+                | t :: ts1 => (is_node n t ∗ branch_node_list ns2 ts1)%I
+                end
+            end) xs ys ∗ is_node xlast ylast).
+    Proof.
+      iIntros "H".
+      iInduction ys as [|y ys] "IH" forall (xs);
+        destruct xs as [|x xs].
+      - iDestruct "H" as "[? _]"; iFrame.
+      - destruct xs; cbn; iDestruct "H" as "[_ ?]"; done.
+      - destruct ys; cbn; iDestruct "H" as "[_ ?]"; done.
+      - iDestruct "H" as "[Hxy H]".
+        iEval (fold (@app val); fold (@app nary_tree)) in "H".
+        iFrame.
+        iApply ("IH" with "H").
+    Qed.
+
+    Lemma branch_node_snoc' xs xlast ys ylast :
+      (fix branch_node_list (ns1 : list val) (ts0 : list nary_tree) {struct ts0} :
+        iProp :=
+         match ns1 with
+         | [] => match ts0 with
+                | [] => True%I
+                | _ :: _ => False%I
+                end
+         | n :: ns2 =>
+             match ts0 with
+             | [] => False%I
+             | t :: ts1 => (is_node n t ∗ branch_node_list ns2 ts1)%I
+             end
+         end) xs ys ∗ is_node xlast ylast -∗
+        (fix branch_node_list (ns1 : list val) (ts0 : list nary_tree) {struct ts0} :
+          iProp :=
+           match ns1 with
+           | [] => match ts0 with
+                  | [] => True%I
+                  | _ :: _ => False%I
+                  end
+           | n :: ns2 =>
+               match ts0 with
+               | [] => False%I
+               | t :: ts1 => (is_node n t ∗ branch_node_list ns2 ts1)%I
+               end
+           end) (xs ++ [xlast]) (ys ++ [ylast]).
+    Proof.
+      iIntros "H".
+      iInduction ys as [|y ys] "IH" forall (xs);
+        destruct xs as [|x xs].
+      - iDestruct "H" as "[_ ?]"; iFrame.
+      - destruct xs; cbn; iDestruct "H" as "[? _]"; done.
+      - destruct ys; cbn; iDestruct "H" as "[? _]"; done.
+      - iDestruct "H" as "[[Hxy H] Hxylast]".
+        iFrame.
+        iApply ("IH" with "[$]").
+    Qed.
+
+    Lemma hd_map_comm {A B} (f : A -> B) (l : list A) (d : A) (fd : B) :
+      fd = f d -> hd (fd) (map f l) = f (hd d l).
+    Proof. destruct l; [done|auto]. Qed.
+
+    Lemma head_map_comm {A B} (f : A -> B) (l : list A) :
+      head (map f l) = match head l with None => None | Some x => Some (f x) end.
+    Proof. destruct l; [done|auto]. Qed.
+
+    Lemma Listlast_map_comm {A B} (f : A -> B) (l : list A) (d : A) (fd : B) :
+      fd = f d -> List.last (map f l) fd = f (List.last l d).
+    Proof.
+      induction l; [done|].
+      destruct l; [auto|done].
+    Qed.
+
+    Lemma last_map_comm {A B} (f : A -> B) (l : list A) :
+      last (map f l) = match last l with None => None | Some x => Some (f x) end.
+    Proof.
+      induction l; [done|].
+      destruct l; [auto|done].
+    Qed.
+
+    Lemma ge_1_S n :
+      1 <= n -> exists m, n = S m.
+    Proof.
+      clear bpos.
+      intros.
+      destruct n; [lia|exists n; done].
+    Qed.
+
+    Lemma take_b2_cons {A} (l : list A) : b < length l -> (exists x l', take (b/2) l = x :: l').
+    Proof using beven bpos.
+      intro.
+      assert (1 < 2) by lia.
+      specialize (Nat.div_lt b 2 bpos H0) as b2ltb.
+      specialize (take_length l (b/2)) as take_len.
+      specialize (b2ge1 _ beven bpos) as ?.
+      assert (0 < b/2) by lia.
+      destruct (take (b/2) l);
+        [ rewrite nil_length in take_len; lia | eauto ].
+    Qed.
+
+    Lemma take_b2_snoc {A} (l : list A) : b < length l -> (exists x l', take (b/2) l = l' ++ [x]).
+    Proof using beven bpos.
+      intro.
+      assert (1 < 2) by lia.
+      specialize (Nat.div_lt b 2 bpos H0) as b2ltb.
+      specialize (take_length l (b/2)) as take_len.
+      specialize (b2ge1 _ beven bpos) as ?.
+      assert (0 < b/2) by lia.
+      destruct (destruct_list_back (take (b/2) l)) as [[x [init ?]]|];
+        subst; rewrite e in take_len; rewrite e;
+        [ eauto | rewrite nil_length in take_len; lia ].
+    Qed.
+
+    Lemma drop_b2_cons {A} (l : list A) : b < length l -> (exists x l', drop (b/2) l = x :: l').
+    Proof using bpos.
+      intro.
+      assert (1 < 2) by lia.
+      specialize (Nat.div_lt b 2 bpos H0) as b2ltb.
+      specialize (drop_length l (b/2)) as drop_len.
+      destruct (drop (b/2) l);
+        [ rewrite nil_length in drop_len; lia | eauto ].
+    Qed.
+
+    Lemma drop_b2_snoc {A} (l : list A) : b < length l -> (exists x l', drop (b/2) l = l' ++ [x]).
+    Proof using bpos.
+      intro.
+      assert (1 < 2) by lia.
+      specialize (Nat.div_lt b 2 bpos H0) as b2ltb.
+      specialize (drop_length l (b/2)) as drop_len.
+      destruct (destruct_list_back (drop (b/2) l)) as [[x [init ?]]|];
+        subst; rewrite e in drop_len; rewrite e;
+        [ eauto | rewrite nil_length in drop_len; lia ].
+    Qed.
+
+    Lemma cons_snoc {A} (l : list A) head tail : l = head :: tail -> exists init last, l = init ++ [last].
+    Proof.
+      destruct (destruct_list_back l) as [[last [init ?]]|];
+        intro; subst;
+        [exists init, last|]; done.
+    Qed.
+
+    Lemma Z2N_b2 : Z.div b 2 = Z.of_nat (b / 2).
+    Proof. symmetry; apply Znat.Nat2Z.inj_div. Qed.
+
     Lemma insert_nary_tree_spec_proof (t : nary_tree) (t_wf : nary_tree_wf_no_len b t) (v : val) (target : tval) :
       {{{ is_node v t }}}
         insert_nary_tree (v, #target)%V
@@ -455,14 +836,14 @@ Section bplus_tree.
                      ∃ (r2 : val), ⌜r.2 = SOMEV r2⌝ ∗ is_node r2 t2) ∨
                  (⌜(insert_nary_tree_spec target t).2 = None⌝ ∗ ⌜r.2 = NONEV⌝))
         }}}.
-    Proof using bpos.
+    Proof using bpos beven.
       iIntros (Φ) "Hv HPost".
 
       iInduction t as [(low & high)|(low & high) ts] "IH" using nary_tree_ind' forall (Φ v).
       - iPoseProof (tree_leaf_token_leaf with "Hv") as (?) "->".
         iDestruct "Hv" as (? ?) "(% & Hptr & Hlhd)".
         assert (x = #ptr) by (unfold token_leaf_v in H; congruence); subst; clear H.
-        wp_rec; wp_load; wp_pures; wp_bind (insert_list _).
+        wp_rec; wp_load; wp_load; wp_pures; wp_bind (insert_list _).
         iApply (insert_list_spec_proof with "Hlhd").
         iNext.
         iIntros (?) "Hr".
@@ -472,33 +853,72 @@ Section bplus_tree.
         iIntros (?) "[% Hr]".
         wp_pure.
         destruct (bool_decide (Z.lt b r0)) eqn:?.
-        + wp_pure; wp_bind (split_list _); wp_pure.
-          replace (Z.div b 2) with (Z.of_nat (b `div` 2)); [|admit]. (* TODO: just annoying arithmetic *)
-          iApply (split_list_spec_proof with "Hr").
-          iNext.
-          iIntros (?) "[Hr1 Hr2]".
-          wp_load; wp_alloc ptr' as "Hptr'"; wp_load; wp_store; wp_pures.
+        + wp_pures.
+          rewrite Z2N_b2.
+          wp_bind (split_list _);
+            iApply (split_list_spec_proof with "Hr");
+            iNext;
+            iIntros (?) "[Hr1 Hr2]".
+          wp_pures;
+            wp_bind (head_list _);
+            iApply (head_list_spec_proof with "Hr1");
+            iNext;
+            iIntros (?) "[-> Hr1]".
+          wp_pures;
+            wp_bind (last_list _);
+            iApply (last_list_spec_proof with "Hr1");
+            iNext;
+            iIntros (?) "[-> Hr1]".
+          wp_pures;
+            wp_bind (head_list _);
+            iApply (head_list_spec_proof with "Hr2");
+            iNext;
+            iIntros (?) "[-> Hr2]".
+          wp_pures;
+            wp_bind (last_list _);
+            iApply (last_list_spec_proof with "Hr2");
+            iNext;
+            iIntros (?) "[-> Hr2]".
+
+          wp_alloc ptr' as "Hptr'"; wp_store; wp_pures.
           iApply ("HPost" $! (InjLV #ptr, InjRV (InjLV #ptr'))).
           rewrite map_length in H; subst r0.
           rewrite bool_decide_eq_true in Heqb0;
             apply Z.ltb_lt in Heqb0.
+          repeat rewrite firstn_map;
+            repeat rewrite skipn_map;
+            rewrite (hd_map_comm _ _ low _ eq_refl);
+            rewrite (Listlast_map_comm _ _ high _ eq_refl).
           iSplitL "Hptr Hr1".
           { cbn; rewrite Heqb0.
             iExists ptr, r1.1.
             iSplitR; [done|].
-            iSplitL "Hptr"; [done|].
-            rewrite firstn_map; done. }
+            iSplitL "Hptr"; done. }
           iLeft.
-          iExists (leaf (low, high) (drop (b `div` 2) (insert_list_spec target vals))).
-          iSplitR. { cbn; rewrite Heqb0; cbn; done. }
+          remember (insert_list_spec target vals) as new_vals.
+          iExists (leaf (hd low (drop (b/2) new_vals), List.last (drop (b/2) new_vals) high) (drop (b/2) new_vals)).
+          iSplitR; [cbn; rewrite <- Heqnew_vals; rewrite Heqb0; done|].
           iExists (InjLV #ptr').
           iSplitR; [done|].
           iExists ptr', r1.2.
-          rewrite skipn_map.
-          iFrame.
-          done.
+          repeat rewrite firstn_map;
+            repeat rewrite skipn_map;
+            rewrite (hd_map_comm _ _ low _ eq_refl);
+            rewrite (Listlast_map_comm _ _ high _ eq_refl).
+          iFrame; done.
 
-        + wp_load; wp_store; wp_pures.
+        + wp_pures;
+            wp_bind (head_list _);
+            iApply (head_list_spec_proof with "Hr");
+            iNext;
+            iIntros (?) "[-> Hr]".
+          wp_pures;
+            wp_bind (last_list _);
+            iApply (last_list_spec_proof with "Hr");
+            iNext;
+            iIntros (?) "[-> Hr]".
+
+          wp_store; wp_pures.
           iApply ("HPost" $! (token_leaf_v #ptr, NONEV)).
           apply bool_decide_eq_false_1 in Heqb0;
               assert (Z.le r0 b) by lia;
@@ -512,8 +932,9 @@ Section bplus_tree.
           { unfold insert_nary_tree_spec.
             rewrite H0.
             iExists ptr, r.
-            iFrame.
-            done. }
+            rewrite (hd_map_comm _ _ low _ eq_refl);
+              rewrite (Listlast_map_comm _ _ high _ eq_refl).
+            iFrame; done. }
           iRight.
           cbn.
           rewrite H0.
@@ -566,10 +987,7 @@ Section bplus_tree.
                                   | None => [new_t1]
                                   end
                               | t :: (_ :: _) as ts0 =>
-                                  let (low0, high0) :=
-                                    match t with
-                                    | leaf interval _ | node interval _ => interval
-                                    end in
+                                  let (low0, high0) := nary_tree_interval t in
                                   if (low0 <=? target)%Z && (target <=? high0)%Z
                                   then
                                     let (new_t1, new_t2) := insert_nary_tree_spec target t in
@@ -597,16 +1015,11 @@ Section bplus_tree.
                          end
                      | SOME "_" =>
                          let: "thd" := Fst !"l" in
-                         let: "interval" :=
-                           match: "thd" with
-                             InjL "ptr" => Fst !"ptr"
-                           | InjR "ptr" => Fst !"ptr"
-                           end in
+                         let: "interval" := interval_nary_tree "thd" in
                          let: "low" := Fst "interval" in
                          let: "high" := Snd "interval" in
                          (if: (BinOp LeOp "low" "target") && (BinOp LeOp "target" "high")
                           then let: "newt" := insert_nary_tree ("thd", "target") in
-                               (* TODO: should change interval here *)
                                match: Snd "newt" with
                                  NONE => "l" <- (Fst "newt", Snd !"l")
                                | SOME "newt2" =>
@@ -662,82 +1075,84 @@ Section bplus_tree.
             + iDestruct "Hlhd" as (l1 ?) "(-> & Hl1 & Hhd')".
               iDestruct "Hhd'" as (l2 ?) "(-> & Hl2 & Hhd')".
               wp_load; wp_load; wp_pures.
-              destruct thd.
-              * destruct interval as [low' high'].
-                iDestruct "Hnhd" as (ptr' leaves) "(-> & Hptr' & Hleaves)".
-                wp_load; wp_pures.
-                destruct (bool_decide (Z.le low' target)) eqn:?; wp_pures.
-                -- destruct (bool_decide (Z.le target high')) eqn:?; wp_pures.
-                   ++ wp_bind (insert_nary_tree _).
-                      iApply ("IHthd" $! thd_wf with "[Hptr' Hleaves]").
-                      { iExists ptr', leaves; iFrame; done. }
-                      iNext.
+              wp_bind (interval_nary_tree _);
+                iApply (interval_nary_tree_spec_proof with "Hnhd");
+                iNext;
+                iIntros ((low', high')) "[Hnhd %]";
+                destruct H0.
+
+              wp_pures.
+              destruct (bool_decide (Z.le low' target)) eqn:?; wp_pures.
+              -- destruct (bool_decide (Z.le target high')) eqn:?; wp_pures.
+                 ++ wp_bind (insert_nary_tree _);
+                      iApply ("IHthd" $! thd_wf with "Hnhd");
+                      iNext;
                       iIntros (?) "[Hr1 Hr2]".
-                      apply bool_decide_eq_true_1 in Heqb0;
-                           apply Z.leb_le in Heqb0;
-                           rewrite Heqb0.
-                         apply bool_decide_eq_true_1 in Heqb1;
-                           apply Z.leb_le in Heqb1;
-                           rewrite Heqb1.
-                      iDestruct "Hr2" as "[(% & % & % & -> & Hr2) | (% & ->)]";
-                        destruct (insert_nary_tree_spec target (leaf (low', high') l)) as [new_t1 new_t2];
-                        cbn in H0; subst.
-                      ** wp_load; wp_alloc l3 as "Hl3"; wp_store; wp_pure.
-                         iApply "HPost".
-                         iExists (r.1 :: r2 :: nsnd :: nrest).
-                         iSplitL "Hl1 Hl3 Hl2 Hhd'";
-                           [iExists l1, (SOMEV #l3); iFrame; iSplitR; [done|]; iExists l3, (SOMEV #l2); iFrame; iSplitR; [done|]; iExists l2, hd'0; iFrame; done|].
-                         iFrame; done.
-                      ** wp_load; wp_store; wp_pure.
-                         iApply "HPost".
-                         iExists (r.1 :: nsnd :: nrest).
-                         iSplitL "Hl1 Hl2 Hhd'";
-                           [iExists l1, (SOMEV #l2); iFrame; iSplitR; [done|]; iExists l2, hd'0; iFrame; done|].
-                         iFrame; done.
-                   ++ wp_load; wp_pure; wp_pure.
-                      wp_bind ((rec: "insert_node_list" "arg" := _) (SOMEV #l2, #target))%V.
-                      iApply ("IH'" $! trest_wf _ (nsnd :: nrest) (SOMEV #l2) with "[] [Hl2 Hhd'] [Hnrest]"); try done.
-                      { iExists l2, hd'0; iFrame; done. }
-                      iIntros (?) "[% [Hr Hns]]".
-                      wp_store; wp_pure.
-                      iApply "HPost".
-                      apply bool_decide_eq_true_1 in Heqb0;
-                        apply Z.leb_le in Heqb0;
-                        rewrite Heqb0.
-                      apply bool_decide_eq_false_1 in Heqb1;
-                        assert (Z.lt high' target) by lia;
-                        apply Z.ltb_lt in H0;
-                        rewrite Z.ltb_antisym in H0;
-                        symmetry in H0;
-                        apply negb_sym in H0;
-                        cbn in H0;
-                        rewrite H0.
-                      iExists (token_leaf_v #ptr' :: ns).
-                      iFrame.
-                      iSplitL "Hl1 Hr"; [iExists l1, r; iFrame; done|].
-                      iExists ptr', leaves; iFrame; done.
-                -- wp_load; wp_pure; wp_pure;
-                     wp_bind ((rec: "insert_node_list" "arg" := _) (SOMEV #l2, #target))%V.
-                   iApply ("IH'" $! trest_wf _ (nsnd :: nrest) with "[] [Hl2 Hhd'] [Hnrest]"); try done.
-                   { iExists l2, hd'0; iFrame; done. }
-                   iIntros (?) "[% [Hr Hns]]".
-                   wp_store; wp_pures.
-                   iApply "HPost".
+                    wp_pures.
+                    apply bool_decide_eq_true_1 in Heqb0;
+                      apply Z.leb_le in Heqb0;
+                      rewrite Heqb0.
+                    apply bool_decide_eq_true_1 in Heqb1;
+                      apply Z.leb_le in Heqb1;
+                      rewrite Heqb1.
 
-                   apply bool_decide_eq_false_1 in Heqb0;
-                     assert (Z.lt target low') by lia;
-                     apply Z.ltb_lt in H0;
-                     rewrite Z.ltb_antisym in H0;
-                     symmetry in H0;
-                     apply negb_sym in H0;
-                     cbn in H0;
-                     rewrite H0.
-                   iExists (token_leaf_v #ptr' :: ns).
-                   iFrame.
-                   iSplitL "Hl1 Hr"; [iExists l1, r; iFrame; done|].
-                   iExists ptr', leaves; iFrame; done.
+                    iDestruct "Hr2" as "[(% & % & % & -> & Hr2) | (% & ->)]";
+                      destruct (insert_nary_tree_spec target thd) as [new_t1 new_t2];
+                      cbn in H0; subst.
+                    ** wp_load; wp_alloc l3 as "Hl3"; wp_store; wp_pure.
+                       iApply "HPost".
+                       iExists (r.1 :: r2 :: nsnd :: nrest).
+                       iSplitL "Hl1 Hl3 Hl2 Hhd'";
+                         [iExists l1, (SOMEV #l3); iFrame; iSplitR; [done|]; iExists l3, (SOMEV #l2); iFrame; iSplitR; [done|]; iExists l2, hd'0; iFrame; done|].
+                       iFrame; done.
+                    ** wp_load; wp_store; wp_pure.
+                       iApply "HPost".
+                       iExists (r.1 :: nsnd :: nrest).
+                       iSplitL "Hl1 Hl2 Hhd'";
+                         [iExists l1, (SOMEV #l2); iFrame; iSplitR; [done|]; iExists l2, hd'0; iFrame; done|].
+                       iFrame; done.
 
-              * admit. (* TODO: repeat for node (or find a better way to get interval out) *) }
+                 ++ wp_load; wp_pure; wp_pure.
+                    wp_bind ((rec: "insert_node_list" "arg" := _) (SOMEV #l2, #target))%V.
+                    iApply ("IH'" $! trest_wf _ (nsnd :: nrest) (SOMEV #l2) with "[] [Hl2 Hhd'] [Hnrest]"); try done.
+                    { iExists l2, hd'0; iFrame; done. }
+                    iIntros (?) "[% [Hr Hns]]".
+                    wp_store; wp_pure.
+                    iApply "HPost".
+                    apply bool_decide_eq_true_1 in Heqb0;
+                      apply Z.leb_le in Heqb0;
+                      rewrite Heqb0.
+                    apply bool_decide_eq_false_1 in Heqb1;
+                      assert (Z.lt high' target) by lia;
+                      apply Z.ltb_lt in H0;
+                      rewrite Z.ltb_antisym in H0;
+                      symmetry in H0;
+                      apply negb_sym in H0;
+                      cbn in H0;
+                      rewrite H0.
+                    iExists (nhd :: ns).
+                    iFrame.
+                    iExists l1, r; iFrame; done.
+
+              -- wp_load; wp_pure; wp_pure;
+                   wp_bind ((rec: "insert_node_list" "arg" := _) (SOMEV #l2, #target))%V.
+                 iApply ("IH'" $! trest_wf _ (nsnd :: nrest) with "[] [Hl2 Hhd'] [Hnrest]"); try done.
+                 { iExists l2, hd'0; iFrame; done. }
+                 iIntros (?) "[% [Hr Hns]]".
+                 wp_store; wp_pures.
+                 iApply "HPost".
+
+                 apply bool_decide_eq_false_1 in Heqb0;
+                   assert (Z.lt target low') by lia;
+                   apply Z.ltb_lt in H0;
+                   rewrite Z.ltb_antisym in H0;
+                   symmetry in H0;
+                   apply negb_sym in H0;
+                   cbn in H0;
+                   rewrite H0.
+                 iExists (nhd :: ns).
+                 iFrame.
+                 iExists l1, r; iFrame; done. }
 
         iClear "IH".
         iApply ("IH'" with "[Hlhd Hns]"); iClear "IH'".
@@ -745,11 +1160,23 @@ Section bplus_tree.
         iIntros (r) "Hr".
         iDestruct "Hr" as (?) "[Hr Hns0]".
 
-        wp_pures; wp_bind (length_list _).
+        wp_load; wp_pures; wp_bind (length_list _).
         iApply (length_list_spec_proof with "Hr").
         iNext.
         iIntros (?) "[% Hr]".
         wp_pure.
+        remember (fix branch_node_list (ns1 : list val) (ts0 : list nary_tree) {struct ts0} : iProp :=
+                 match ns1 with
+                 | [] => match ts0 with
+                         | [] => True
+                         | _ :: _ => False
+                         end
+                 | n :: ns2 =>
+                     match ts0 with
+                     | [] => False
+                     | t :: ts1 => is_node n t ∗ branch_node_list ns2 ts1
+                     end
+                 end)%I as branch_node_list.
         remember ((fix insert_aux (l : list nary_tree) : list nary_tree :=
                      match l with
                      | [] => []
@@ -760,10 +1187,7 @@ Section bplus_tree.
                          | None => [new_t1]
                          end
                      | t :: (_ :: _) as ts0 =>
-                         let (low0, high0) :=
-                           match t with
-                           | leaf interval _ | node interval _ => interval
-                           end in
+                         let (low0, high0) := nary_tree_interval t in
                          if (low0 <=? target)%Z && (target <=? high0)%Z
                          then
                            let (new_t1, new_t2) := insert_nary_tree_spec target t in
@@ -774,51 +1198,266 @@ Section bplus_tree.
                          else t :: insert_aux ts0
                      end) ts) as new_ts.
         destruct (bool_decide (Z.lt b r0)) eqn:?.
-        + wp_pure; wp_bind (split_list _); wp_pure.
-          replace (Z.div b 2) with (Z.of_nat (b `div` 2)); [|admit]. (* TODO: just annoying arithmetic *)
+        + wp_pures; wp_bind (split_list _).
+          rewrite Z2N_b2.
           iApply (split_list_spec_proof with "Hr").
           iNext.
           iIntros (?) "[Hr1 Hr2]".
-          wp_load; wp_alloc ptr' as "Hptr'"; wp_load; wp_store; wp_pures.
-          iApply ("HPost" $! (token_branch_v #ptr, token_branch_v (SOMEV #ptr'))).
-          subst r0.
-          rewrite bool_decide_eq_true in Heqb0;
-            apply Z.ltb_lt in Heqb0.
-          iPoseProof ((branch_node_list_lengths ns0 new_ts) with "Hns0") as "[Hns0 %Heqlengths]".
-          rewrite <- Heqlengths, Heqb0.
-          iPoseProof ((branch_node_split ns0 new_ts (b/2)) with "Hns0") as "[Htakens Hdropns]".
 
-          iSplitL "Hptr Hr1 Htakens".
-          { cbn.
-            iExists ptr, r1.1, (take (b/2) ns0).
-            iFrame.
-            done. }
+          iPoseProof ((branch_node_list_lengths ns0 new_ts) with "[Hns0]") as "[Hns0 %Heqlengths]";
+            [rewrite Heqbranch_node_list; done|].
+          iPoseProof ((branch_node_split (b/2)) with "Hns0") as "[Hnstake Hnsdrop]";
+            iEval (rewrite <- Heqbranch_node_list) in "Hnstake Hnsdrop".
+          assert (b < length new_ts) as bltlengthnew_ts by (rewrite bool_decide_eq_true in Heqb0; lia);
+            specialize (take_b2_cons new_ts bltlengthnew_ts) as [tthd [ttrest take_new_ts_cons]];
+            specialize (take_b2_snoc new_ts bltlengthnew_ts) as [ttlast [ttrest' take_new_ts_snoc]];
+            specialize (drop_b2_cons new_ts bltlengthnew_ts) as [dthd [dtrest drop_new_ts_cons]];
+            specialize (drop_b2_snoc new_ts bltlengthnew_ts) as [dtlast [dtrest' drop_new_ts_snoc]];
+            clear bltlengthnew_ts.
+          assert (b < length ns0) as bltlengthns0 by (rewrite bool_decide_eq_true in Heqb0; lia);
+            specialize (take_b2_cons ns0 bltlengthns0) as [tnhd [tnrest take_ns0_cons]];
+            specialize (take_b2_snoc ns0 bltlengthns0) as [tnlast [tnrest' take_ns0_snoc]];
+            specialize (drop_b2_cons ns0 bltlengthns0) as [dnhd [dnrest drop_ns0_cons]];
+            specialize (drop_b2_snoc ns0 bltlengthns0) as [dnlast [dnrest' drop_ns0_snoc]].
+
+          wp_pures;
+            wp_bind (headopt_list _);
+            iApply (headopt_list_spec_proof with "Hr1");
+            iNext;
+            iIntros (?) "[-> Hr1]";
+            rewrite take_new_ts_cons;
+            rewrite take_ns0_cons;
+            wp_pures;
+            wp_bind (interval_nary_tree _);
+            iEval (rewrite Heqbranch_node_list) in "Hnstake";
+            iDestruct "Hnstake" as "[Htnhd Htnsrest]";
+            iApply (interval_nary_tree_spec_proof with "Htnhd");
+            iNext;
+            iIntros ((thdlow, thdhigh)) "[Htnhd %]";
+            iCombine "Htnhd Htnsrest" as "Hnstake";
+            assert (is_node tnhd tthd ∗ branch_node_list tnrest ttrest -∗
+                      branch_node_list (tnhd :: tnrest) (tthd :: ttrest)) as Heqnstake
+            by (rewrite Heqbranch_node_list; done);
+            iPoseProof (Heqnstake with "[Hnstake]") as "Hnstake"; [rewrite Heqbranch_node_list; iFrame|];
+            rewrite <- take_new_ts_cons;
+            rewrite <- take_ns0_cons.
+
+          wp_pures;
+            wp_bind (lastopt_list _);
+            iApply (lastopt_list_spec_proof with "Hr1");
+            iNext;
+            iIntros (?) "[-> Hr1]";
+            rewrite take_new_ts_snoc;
+            rewrite take_ns0_snoc;
+            wp_pures;
+            iEval (rewrite last_snoc);
+            wp_pures;
+            wp_bind (interval_nary_tree _);
+            iEval (rewrite Heqbranch_node_list) in "Hnstake";
+            iDestruct (branch_node_snoc with "Hnstake") as "[Htnsrest Htnlast]";
+            iApply (interval_nary_tree_spec_proof with "Htnlast");
+            iNext;
+            iIntros ((tlastlow, tlasthigh)) "[Htnlast %]";
+            iCombine "Htnsrest Htnlast" as "Hnstake";
+            iPoseProof (branch_node_snoc' with "[Hnstake]") as "Hnstake"; [iFrame|];
+            iEval (rewrite <- Heqbranch_node_list) in "Hnstake";
+            rewrite <- take_new_ts_snoc;
+            rewrite <- take_ns0_snoc.
+
+          wp_pures;
+            wp_bind (headopt_list _);
+            iApply (headopt_list_spec_proof with "Hr2");
+            iNext;
+            iIntros (?) "[-> Hr2]";
+            rewrite drop_new_ts_cons;
+            rewrite drop_ns0_cons;
+            wp_pures;
+            wp_bind (interval_nary_tree _);
+            iEval (rewrite Heqbranch_node_list) in "Hnsdrop";
+            iDestruct "Hnsdrop" as "[Hdnhd Hdnsrest]";
+            iApply (interval_nary_tree_spec_proof with "Hdnhd");
+            iNext;
+            iIntros ((dthdlow, dthdhigh)) "[Hdnhd %]";
+            iCombine "Hdnhd Hdnsrest" as "Hnsdrop";
+            assert (is_node dnhd dthd ∗ branch_node_list dnrest dtrest -∗
+                      branch_node_list (dnhd :: dnrest) (dthd :: dtrest)) as Heqnsdrop
+              by (rewrite Heqbranch_node_list; done);
+            iPoseProof (Heqnsdrop with "[Hnsdrop]") as "Hnsdrop";
+              [rewrite Heqbranch_node_list; iFrame|];
+            rewrite <- drop_new_ts_cons;
+            rewrite <- drop_ns0_cons.
+
+          wp_pures;
+            wp_bind (lastopt_list _);
+            iApply (lastopt_list_spec_proof with "Hr2");
+            iNext;
+            iIntros (?) "[-> Hr2]";
+            rewrite drop_new_ts_snoc;
+            rewrite drop_ns0_snoc;
+            wp_pures;
+            iEval (rewrite last_snoc);
+            wp_pures;
+            wp_bind (interval_nary_tree _);
+            iEval (rewrite Heqbranch_node_list) in "Hnsdrop";
+            iDestruct (branch_node_snoc with "Hnsdrop") as "[Hnsrest Hnlast]";
+            iApply (interval_nary_tree_spec_proof with "Hnlast");
+            iNext;
+            iIntros ((dtlastlow, dtlasthigh)) "[Hnlast %]";
+            iCombine "Hnsrest Hnlast" as "Hnsdrop";
+            iPoseProof (branch_node_snoc' with "Hnsdrop") as "Hnsdrop";
+            rewrite <- drop_new_ts_snoc;
+            rewrite <- drop_ns0_snoc.
+
+          wp_pures; wp_alloc ptr' as "Hptr'"; wp_store; wp_pures.
+          iApply ("HPost" $! (token_branch_v #ptr, token_branch_v (SOMEV #ptr'))).
+          subst r0;
+            rewrite bool_decide_eq_true in Heqb0;
+            apply Z.ltb_lt in Heqb0;
+            rewrite <- Heqlengths, Heqb0.
+
+          iSplitL "Hptr Hr1 Hnstake".
+          { iExists ptr, r1.1, (take (b/2) ns0).
+            fold is_node; rewrite <- Heqbranch_node_list.
+            repeat rewrite head_map_comm last_map_comm.
+            rewrite take_new_ts_cons;
+              rewrite take_ns0_cons;
+              iEval (rewrite head_cons);
+              rewrite <- take_new_ts_cons;
+              rewrite <- take_ns0_cons.
+            rewrite take_new_ts_snoc;
+              rewrite take_ns0_snoc;
+              iEval (rewrite last_snoc);
+              rewrite <- take_new_ts_snoc;
+              rewrite <- take_ns0_snoc.
+            destruct H1, H2.
+            iFrame; done. }
+
           iLeft.
-          iExists (node (low, high) (drop (b/2) new_ts)).
+          repeat rewrite head_map_comm last_map_comm.
+          rewrite <- Heqbranch_node_list.
+          rewrite drop_new_ts_cons;
+            rewrite drop_ns0_cons;
+            iEval (rewrite head_cons);
+            rewrite <- drop_new_ts_cons;
+            rewrite <- drop_ns0_cons.
+          rewrite drop_new_ts_snoc;
+            rewrite drop_ns0_snoc;
+            iEval (rewrite last_snoc);
+            rewrite <- drop_new_ts_snoc;
+            rewrite <- drop_ns0_snoc.
+
+          iExists (node (fst (nary_tree_interval dthd), snd (nary_tree_interval dtlast)) (drop (b/2) new_ts)).
           iSplitR; [done|].
           iExists (token_branch_v #ptr').
           iSplitR; [done|].
           iExists ptr', r1.2, (drop (b/2) ns0).
-          iFrame.
-          done.
+          fold is_node.
+          rewrite <- Heqbranch_node_list.
+          destruct H3, H4.
+          iFrame; done.
 
-        + wp_load; wp_store; wp_pures.
-          iApply ("HPost" $! (token_branch_v #ptr, NONEV)).
-          apply bool_decide_eq_false_1 in Heqb0;
-            assert (Z.le r0 b) by lia;
-            apply Z.leb_le in H1;
-            rewrite Z.leb_antisym in H1;
-            symmetry in H1;
-            apply negb_sym in H1;
-            cbn in H1.
-          subst r0.
-          iPoseProof ((branch_node_list_lengths ns0 new_ts) with "Hns0") as "[Hns0 %Heqlengths]".
-          rewrite <- Heqlengths, H1.
+        + iPoseProof ((branch_node_list_lengths ns0 new_ts) with "[Hns0]") as "[Hns %Heqlengths]";
+            [rewrite Heqbranch_node_list; done|];
+            rewrite <- Heqbranch_node_list.
 
-          iSplitL "Hptr Hr Hns0"; [iExists ptr, r, ns0; iFrame; done|].
-          iRight.
-          done.
-    Admitted.
+          destruct new_ts as [|thd trest];
+            destruct ns0 as [|nhd nrest];
+            [|rewrite Heqbranch_node_list; done|rewrite Heqbranch_node_list; done|].
+          * wp_pures;
+              wp_bind (headopt_list _);
+              iApply (headopt_list_spec_proof with "Hr");
+              iNext;
+              iIntros (?) "[-> Hr]";
+              iEval (rewrite head_nil).
+
+            wp_pures;
+              wp_bind (lastopt_list _);
+              iApply (lastopt_list_spec_proof with "Hr");
+              iNext;
+              iIntros (?) "[-> Hr]";
+              iEval (rewrite last_nil).
+
+            wp_store; wp_pures.
+
+            iApply ("HPost" $! (token_branch_v #ptr, NONEV)).
+            apply bool_decide_eq_false_1 in Heqb0;
+              assert (Z.le r0 b) by lia;
+              apply Z.leb_le in H1;
+              rewrite Z.leb_antisym in H1;
+              symmetry in H1;
+              apply negb_sym in H1;
+              cbn in H1;
+              subst r0;
+              rewrite H1.
+
+            iSplitL; [iExists ptr, r, []; iFrame; done|].
+            iRight.
+            done.
+
+          * wp_pures;
+              wp_bind (headopt_list _);
+              iApply (headopt_list_spec_proof with "Hr");
+              iNext;
+              iIntros (?) "[-> Hr]";
+              iEval (rewrite head_cons);
+              wp_pures;
+              wp_bind (interval_nary_tree _);
+              iEval (rewrite Heqbranch_node_list) in "Hns";
+              iDestruct "Hns" as "[Hnhd Hnsrest]";
+              iApply (interval_nary_tree_spec_proof with "Hnhd");
+              iNext;
+              iIntros ((hdlow, hdhigh)) "[Hnhd %]";
+              iCombine "Hnhd Hnsrest" as "Hns";
+              assert (is_node nhd thd ∗ branch_node_list nrest trest -∗
+                        branch_node_list (nhd :: nrest) (thd :: trest)) as Heqnbranches
+                by (rewrite Heqbranch_node_list; done);
+              iPoseProof (Heqnbranches with "[Hns]") as "Hns";
+              [rewrite Heqbranch_node_list; iFrame|].
+
+            destruct (cons_snoc (thd :: trest) _ _ eq_refl) as [tlast [tinit Heqts]].
+            destruct (cons_snoc (nhd :: nrest) _ _ eq_refl) as [nlast [ninit Heqns]].
+
+            rewrite Heqts Heqns;
+              wp_pures;
+              wp_bind (lastopt_list _);
+              iApply (lastopt_list_spec_proof with "Hr");
+              iNext;
+              iIntros (?) "[-> Hr]";
+              iEval (rewrite last_snoc);
+              wp_pures;
+              wp_bind (interval_nary_tree _);
+              iEval (rewrite Heqbranch_node_list) in "Hns";
+              iDestruct (branch_node_snoc with "Hns") as "[Hnsrest Hnlast]";
+              iApply (interval_nary_tree_spec_proof with "Hnlast");
+              iNext;
+              iIntros ((lastlow, lasthigh)) "[Hnlast %]";
+              iCombine "Hnsrest Hnlast" as "Hns";
+              iPoseProof (branch_node_snoc' with "Hns") as "Hns";
+              rewrite <- Heqts, <- Heqns.
+
+            wp_store; wp_pures.
+            iApply ("HPost" $! (token_branch_v #ptr, NONEV)).
+            apply bool_decide_eq_false_1 in Heqb0;
+              assert (Z.le r0 b) by lia;
+              apply Z.leb_le in H3;
+              rewrite Z.leb_antisym in H3;
+              symmetry in H3;
+              apply negb_sym in H3;
+              cbn in H3;
+              rewrite <- Heqlengths;
+              subst r0;
+              rewrite H3.
+
+            repeat rewrite head_map_comm last_map_comm;
+              rewrite head_cons;
+              rewrite Heqts;
+              rewrite last_snoc;
+              rewrite <- Heqts.
+
+            destruct H1, H2.
+            iSplitL; [iExists ptr, r, (nhd :: nrest); iFrame; done|].
+            iRight; done.
+    Qed.
 
   End bplus_tree_proofs.
 End bplus_tree.
